work on factorial

examples/Factorial.v
@@ -1,3 +1,4 @@
+(* begin hide *)
 Set Implicit Arguments.
 Set Contextual Implicit.
 
@@ -19,6 +20,10 @@ From ITree Require Import
 
 Import MonadNotation.
 Open Scope monad_scope.
+
+(* end hide *)
+
+(** * Factorial *)
 
 (** This file gives and example of defining a recursive version of the "factorial" 
     function using ITrees. It demonstrates
@@ -42,10 +47,10 @@ Open Scope monad_scope.
 
 (** We write the body of the function monadically, using events rather than recursive calls. *)
 Definition fact_body {E}  : nat -> itree (callE nat nat +' E) nat :=
-  (fun x => match x with
-         | 0 => Ret 1
-         | S m => y <- call m ;; Ret (x * y)
-         end).
+  fun x => match x with
+        | 0 => Ret 1
+        | S m => y <- call m ;; Ret (x * y)
+        end.
 
 (** The factorial function itself is defined as an itree by 'tying the knot' using [rec]. 
 
@@ -55,26 +60,22 @@ Definition factorial {E} (n:nat) : itree E nat :=
   rec fact_body n.
 
 (** This is the Coq specification -- the usual mathematical definition. *)
-Fixpoint factspec (n:nat) : nat :=
+Fixpoint factorial_spec (n:nat) : nat :=
   match n with
   | 0 => 1
-  | S m => n * factspec m
+  | S m => n * factorial_spec m
   end.
 
 (** We can prove that the ITrees version [factorial] is "equivalent" to the
-    [factspec] version.  The proof goes by induction on n and uses only
+    [factorial_spec] version.  The proof goes by induction on n and uses only
     rewriting -- no coinduction necessary. Here, we step through each step of
     rewriting to illustrate the use of the equational theory, which is mostly
     applications of the monad laws and the properties of [rec], seen as an 
     instance of [mrec]. 
+
+    In this proof, we do all of the rewriting steps explicitly.
 *)
-(* SAZ: The rewriting in this proof is a bit annoying.  
-    - We have to use itree_eta in order to rewrite with ret_bind.  
-    - the use of cbn to drive the interp forward also unfolds the fact_body too
-      much, which means we have to use fold_bind so that interp_bind can see
-      the bind.
-*)
-Lemma factorial_correct : forall {E} n, (factorial n : itree E nat) ≈ Ret (factspec n).
+Lemma factorial_correct : forall {E} n, (factorial n : itree E nat) ≈ Ret (factorial_spec n).
 Proof.
   intros E n.
   induction n; intros; subst.
@@ -89,23 +90,222 @@ Proof.
 Qed.
 
 
-(* HIDE *)
-(* SAZ: we might experiment with automating monadic rewriting according to the equational reasoning, 
-   something like: *)
-Ltac simpl_monad :=
-    repeat match goal with
-           | [ |- context[Tau ?T] ] => progress rewrite tau_eutt
-           | [ |- context[ITree.bind (Ret ?X) ?K] ] => progress rewrite ret_bind
-           | [ |- context[interp_mrec _ _ (ITree.bind ?T ?K)] ] => progress rewrite interp_mrec_bind
-           | [ |- context[interp_mrec _ _ (Ret ?X)] ] => progress rewrite ret_mrec                                                                         
-           end.
-                     
-(* Then the proof above becomes: 
+(** * Fibonacci *)
 
-    simpl_monad.
-    rewrite IHn.
-    simpl_monad.
-    reflexivity.
-*)
-(* /HIDE *)
+(** Exercise *)
+(** Carry out the analogous proof of correctness for the Fibonacci function, whose
+    naturally recursive coq definition is given below. *)
+
+Fixpoint fib_spec (n:nat) : nat :=
+  match n with
+  | 0 => 1
+  | S m =>
+    match m with
+    | 0 => 1
+    | S k => fib_spec m + fib_spec k
+    end
+  end.
+
+(** We write the body of the fib monadically, using events rather than recursive calls. *)
+Definition fib_body {E}  : nat -> itree (callE nat nat +' E) nat :=
+(* SOLN *)  
+  fun x => match x with
+        | 0 => Ret 1
+        | S m =>
+          match m with
+          | 0 => Ret 1
+          | S k => y1 <- call m ;;
+                  y2 <- call k ;;
+                  Ret (y1 + y2)
+          end
+        end.
+(* STUBWITH Ret 0 *)
+
+Require Import Omega.
+
+Definition fib {E} n : itree E nat :=
+  rec fib_body n.
+
+(** Since fib uses two recursive calls, we need to strengthen the induction hypothesis.  One way
+   to do that is to prove the property for all [m <= n]. *)
+(* SAZ: is this a good example? The stronger induction hypothesis is kind of orthogonal to the 
+   point we're trying to make. *)
+Lemma fib_correct : forall {E} n m, m <= n ->
+    (fib m : itree E nat ) ≈ Ret (fib_spec m).
+Proof.
+(* SOLN *)  
+  intros E n.
+  induction n; intros; subst.
+  - apply Le.le_n_0_eq in H. subst. 
+    unfold fib.  rewrite rec_unfold. simpl. rewrite ret_interp.  reflexivity.
+  - induction m; intros; subst.
+    + unfold fib. rewrite rec_unfold. simpl. rewrite ret_interp. reflexivity.
+    + unfold fib.
+      rewrite rec_unfold. simpl.
+      destruct m.
+      * rewrite ret_interp. reflexivity.
+      * rewrite interp_bind. rewrite interp_recursive_call. rewrite IHm.
+        rewrite ret_bind. rewrite interp_bind. rewrite interp_recursive_call.
+        unfold fib in IHn. rewrite IHn. rewrite ret_bind.
+        rewrite ret_interp. reflexivity.
+        omega. omega. 
+Qed.
+(* STUBWITH Admitted. *)
+
+
+Inductive tree (X:Type) :=
+| Empty
+| Node (t1 : tree X) (x:X) (t2 : tree X)
+.
+
+
+Require Import Lists.List.
+Require Import Paco.paco.
+Open Scope list_scope.
+
+
+
+
+Definition bfs_body {E} (n:nat) (q : list (tree nat)) : itree (callE (list (tree nat)) bool +' E) bool :=
+  match q with
+  | [] => Ret false
+  | t::ts => match t with
+           | Empty => call ts
+           | Node t1 x t2 =>
+             if Nat.eqb n x then Ret true else call (ts ++ [t1; t2])
+           end
+  end.
+
+Definition bfs {E} n (t:tree nat) : itree E bool :=
+  rec (bfs_body n) [t].
+
+Definition dfs_body {E} (n:nat) (q : list (tree nat)) : itree (callE (list (tree nat)) bool +' E) bool :=
+  match q with
+  | [] => Ret false
+  | t::ts => match t with
+           | Empty => call ts
+           | Node t1 x t2 =>
+             if Nat.eqb n x then Ret true else call ([t1 ; t2] ++ ts)
+           end
+  end.
+
+Definition dfs {E} n (t:tree nat) : itree E bool :=
+  rec (bfs_body n) [t].
+
+
+
+Lemma bfs_dfs : forall {E} n q, rec (bfs_body n) q ≈ (rec (dfs_body n) q : itree E bool).
+Proof.
+  intros E n q.
+  pupto2_init.
+  revert q.
+  pcofix CIH.
+  intros q.
+  do 2 rewrite rec_unfold.
+  induction q; simpl.
+  - rewrite ret_interp. rewrite ret_interp.  pupto2_final.  pfold.  pfold. econstructor. reflexivity.  (* SAZ This reflexivity proof is annoyting .*)
+  - destruct a.
+    + rewrite interp_recursive_call.  rewrite interp_recursive_call.
+      rewrite rec_unfold. rewrite rec_unfold. assumption.
+    + destruct (n =? x).
+      * rewrite ret_interp. rewrite ret_interp. pupto2_final.  pfold.  pfold. econstructor. reflexivity.  (* SAZ This reflexivity proof is annoyting .*)
+      * rewrite interp_recursive_call.  rewrite interp_recursive_call.
+        
+      
+                              
+
+Lemma bfs_q : forall {E:Type->Type} n t ts,
+                  (rec (bfs_body n) (t::ts) : itree E bool) ≈ match t with
+                                 | Empty => rec (bfs_body n) ts
+                                 | Node t1 x t2 =>
+                                   if Nat.eqb n x then Ret true else rec (bfs_body n) (ts ++ [t1; t2])
+                                                          end.
+Proof.
+  intros.
+  rewrite rec_unfold. simpl.
+  destruct t.
+  rewrite interp_recursive_call. reflexivity.
+  destruct (n =? x).
+  rewrite ret_interp. reflexivity.
+  rewrite interp_recursive_call. reflexivity.
+Qed.
+
+Require Import Lists.List.
+Require Import Paco.paco.
+
+Fixpoint contains n (t:tree nat) : bool :=
+  match t with
+  | Empty => false
+  | Node t1 x t2 => if Nat.eqb n x then true else orb (contains n t1) (contains n t2)
+  end.
+
+Lemma fold_orb_true : forall l : list bool, 
+    fold_left (fun x y => orb x y) l true = true.
+Proof.
+  induction l; auto.
+Qed.
+
+Lemma bfs_contains : forall E n (q : list (tree nat)),
+    (rec (bfs_body n) q : itree E bool) ≈
+        (Ret (List.fold_left (fun x y => orb x y) (List.map (contains n) q) false)).
+Proof.
+  intros E n q.
+  pupto2_init.
+  revert q.
+  pcofix CIH.
+  intros q.
+  induction q; simpl.
+  - rewrite rec_unfold. simpl.  rewrite ret_interp. pupto2_final.  pfold. pfold. econstructor. reflexivity.
+  - rewrite rec_unfold. simpl. destruct a; simpl.
+    + rewrite interp_recursive_call.  assumption.
+    + destruct (n =? x); simpl.
+      * rewrite fold_orb_true.
+        rewrite ret_interp. pupto2_final. pfold. pfold. econstructor. reflexivity.
+      * rewrite interp_recursive_call.
+        
+
+
+Lemma bfs_q2 : forall {E:Type->Type} n q1 q2,
+    (rec (bfs_body n) (q1 ++ q2) : itree E bool) ≈ 
+                                              (y1 <- rec (bfs_body n) q1 ;;
+                                               y2 <- rec (bfs_body n) q2 ;;
+                                               Ret (orb y1 y2)).
+Proof.
+  intros E n.
+  induction q1; intros q2; simpl.
+  - rewrite rec_unfold. rewrite rec_unfold.
+    simpl.  rewrite ret_interp. rewrite ret_bind.
+    rewrite rec_unfold.  simpl. rewrite bind_ret. reflexivity.
+  - do 2 rewrite rec_unfold.
+    simpl.
+    destruct a.
+    + rewrite interp_recursive_call.
+      rewrite IHq1.
+      rewrite interp_recursive_call.
+      reflexivity.
+    + destruct (n =? x).
+      rewrite ret_interp.
+      rewrite ret_bind. simpl. 
+    
+
+  
+
+
+
+Lemma contains_bfs: forall {E} n t, (bfs n t : itree E bool) ≈ Ret (contains t n).
+Proof.
+  intros E n t.
+  pupto2_init.
+  revert n t.
+  pcofix CIH.
+  intros n t.
+  unfold bfs.
+  rewrite bfs_q.
+  destruct t; simpl.
+  - rewrite rec_unfold.  simpl. rewrite ret_interp. pupto2_final. pfold.  pfold. econstructor. reflexivity.
+  - destruct (n=?x).
+    pfold. pfold. econstructor. reflexivity.
+    
+  
+
 
